shorter proof

src/Relations.dfy
@@ -60,37 +60,23 @@ module {:options "-functionSyntax:4"} Relations {
   }
 
   /* An element in an ordered set is called minimal, if it is less than every element of the set. */
-  ghost predicate IsMinimum<T>(R: (T, T) -> bool, m: T, s: set<T>) 
-  {
+  ghost predicate IsMinimum<T>(R: (T, T) -> bool, m: T, s: set<T>) {
     m in s && forall y: T | y in s :: R(m, y)
   }
 
   /* Any totally ordered set contains a unique minimal element. */
-  lemma LemmaUniqueMinimum<T(!new)>(R: (T, T) -> bool, s: set<T>) 
-    requires &&|s| > 0 
-             && TotalOrdering(R)
-    ensures && (exists m: T :: IsMinimum(R, m, s))
-            && (forall m, n: T :: IsMinimum(R, m, s) && IsMinimum(R, n, s) ==> m == n)
+  lemma LemmaUniqueMinimum<T(!new)>(R: (T, T) -> bool, s: set<T>) returns (m: T)
+    requires |s| > 0 && TotalOrdering(R)
+    ensures IsMinimum(R, m, s) && (forall n: T :: IsMinimum(R, n, s) ==> m == n)
   {
     var x :| x in s;
     if s == {x} {
-      assert IsMinimum(R, x, s);
+      m := x;
     } else {
-      var s' := s - {x};
-      LemmaUniqueMinimum(R, s');
-      var z :| IsMinimum(R, z, s');
+      var m' := LemmaUniqueMinimum(R, s - {x});
       if 
-      case R(z, x) => {
-        forall y: T | y in s ensures R(z, y) {
-        }
-        assert IsMinimum(R, z, s); 
-      }
-      case R(x, z) => {
-        forall y: T | y in s ensures R(x, y) {
-        }
-        assert IsMinimum(R, x, s); 
-      }
-    assert exists m: T :: IsMinimum(R, m, s);
+      case R(m', x) => m := m';
+      case R(x, m') => m := x;
     }
   }
 
